src/michocoq/typer.v
@@ -39,7 +39,7 @@ Module Typer(C:ContractContext).
 
   Definition instruction_cast {self_type tff} A A' B B' i : M (instruction self_type tff A' B') :=
     match stype_dec A A', stype_dec B B' with
-    | left HA, left HB => Return _ (safe_instruction_cast A A' B B' i HA HB)
+    | left HA, left HB => Return (safe_instruction_cast A A' B B' i HA HB)
     | _, _ => Failed _ (Typing cast_error (Mk_cast_error A B A' B' tff _ i))
     end.
 
@@ -68,8 +68,8 @@ Module Typer(C:ContractContext).
     match r1 with
     | Inferred_type _ B' i =>
       let! i := instruction_cast_range A B' B i in
-      Return _ (existT _ false i)
-    | Any_type _ i => Return _ (existT _ true (i B))
+      Return (existT _ false i)
+    | Any_type _ i => Return (existT _ true (i B))
     end.
 
   Definition type_check_instruction_no_tail_fail {self_type}
@@ -86,7 +86,7 @@ Module Typer(C:ContractContext).
   Definition assert_not_tail_fail {self_type} A (r : typer_result A) :
     M {B & instruction self_type Datatypes.false A B} :=
     match r with
-    | Inferred_type _ B i => Return _ (existT _ B i)
+    | Inferred_type _ B i => Return (existT _ B i)
     | Any_type _ _ => Failed _ (Typing _ tt)
     end.
 
@@ -113,34 +113,34 @@ Module Typer(C:ContractContext).
     match r1, r2 with
     | Inferred_type _ B1 i1, Inferred_type _ B2 i2 =>
       let! i2 := instruction_cast_range A2 B2 B1 i2 in
-      Return _
+      Return
               (Inferred_type _ _
                             (IF_instr B1 false false i1 i2))
     | Inferred_type _ B i1, Any_type _ i2 =>
-      Return _ (Inferred_type _ _ (IF_instr B false true i1 (i2 B)))
+      Return (Inferred_type _ _ (IF_instr B false true i1 (i2 B)))
     | Any_type _ i1, Inferred_type _ B i2 =>
-      Return _ (Inferred_type _ _ (IF_instr B true false (i1 B) i2))
+      Return (Inferred_type _ _ (IF_instr B true false (i1 B) i2))
     | Any_type _ i1, Any_type _ i2 =>
-      Return _ (Any_type _ (fun B =>
+      Return (Any_type _ (fun B =>
                               IF_instr B true true (i1 B) (i2 B)))
     end.
 
   Definition take_one (S : stack_type) : M (type * stack_type) :=
     match S with
     | nil => Failed _ (Typing _ "take_one"%string)
-    | cons a l => Return _ (a, l)
+    | cons a l => Return (a, l)
     end.
 
   Fixpoint take_n (A : stack_type) n : M ({B | List.length B = n} * stack_type) :=
     match n as n return M ({B | List.length B = n} * stack_type) with
-    | 0 => Return ({B | List.length B = 0} * stack_type) (exist (fun B => List.length B = 0) nil eq_refl, A)
+    | 0 => Return (exist (fun B => List.length B = 0) nil eq_refl, A)
     | S n =>
       let! (a, A) := take_one A in
       let! (exist _ B H, C) := take_n A n in
-      Return _ (exist _ (cons a B) (f_equal S H), C)
+      Return (exist _ (cons a B) (f_equal S H), C)
     end.
 
-  Lemma take_n_length n S1 S2 H1 : take_n (S1 ++ S2) n = Return _ (exist _ S1 H1, S2).
+  Lemma take_n_length n S1 S2 H1 : take_n (S1 ++ S2) n = Return (exist _ S1 H1, S2).
   Proof.
     generalize dependent S1.
     induction n; destruct S1; simpl; intro H1.
@@ -163,25 +163,25 @@ Module Typer(C:ContractContext).
     let! (exist _ S1 H1, tS2) := take_n S n in
     let! (t, S2) := take_one tS2 in
     let! i := instruction_cast_domain (S1 +++ t ::: S2) S _ (syntax.DIG n H1) in
-    Return _ (Inferred_type S (t ::: S1 +++ S2) i).
+    Return (Inferred_type S (t ::: S1 +++ S2) i).
 
   Definition type_check_dug {self_type} n (S:stack_type) : M (typer_result (self_type := self_type) S) :=
     let! (t, S12) := take_one S in
     let! (exist _ S1 H1, S2) := take_n S12 n in
     let! i := instruction_cast_domain (t ::: S1 +++ S2) S _ (syntax.DUG n H1) in
-    Return _ (Inferred_type S (S1 +++ t ::: S2) i).
+    Return (Inferred_type S (S1 +++ t ::: S2) i).
 
   Fixpoint as_comparable (a : type) : M comparable_type :=
     match a with
-    | Comparable_type a => Return _ (Comparable_type_simple a)
+    | Comparable_type a => Return (Comparable_type_simple a)
     | pair (Comparable_type a) b =>
       let! b := as_comparable b in
-      Return _ (Cpair a b)
+      Return (Cpair a b)
     | _ => Failed _ (Typing _ ("not a comparable type"%string, a))
     end.
 
   Lemma as_comparable_comparable (a : comparable_type) :
-    as_comparable a = Return _ a.
+    as_comparable a = Return a.
   Proof.
     induction a.
     - reflexivity.
@@ -194,7 +194,7 @@ Module Typer(C:ContractContext).
     match tyopt return C.get_contract_type c = tyopt -> error.M (syntax.concrete_data (contract a)) with
     | Some b =>
       match type_dec a b with
-      | left He => fun H => Return _ (contract_cast c a b H He)
+      | left He => fun H => Return (contract_cast c a b H He)
       | right _ => fun _ => Failed _ (Typing _ ("ill-typed contract"%string, c, a, b))
       end
     | None => fun _ => Failed _ (Typing _ ("contract not found"%string, c))
@@ -208,52 +208,52 @@ Module Typer(C:ContractContext).
     | Int_constant z =>
       fun ty =>
         match ty with
-        | Comparable_type int => Return _ (syntax.Int_constant z)
+        | Comparable_type int => Return (syntax.Int_constant z)
         | Comparable_type nat =>
-          if (z >=? 0)%Z then Return _ (syntax.Nat_constant (Z.to_N z))
+          if (z >=? 0)%Z then Return (syntax.Nat_constant (Z.to_N z))
           else Failed _ (Typing _ ("Negative value cannot be typed in nat"%string, d))
         | Comparable_type mutez =>
           let! m := tez.of_Z z in
-          Return _ (syntax.Mutez_constant (Mk_mutez m))
-        | Comparable_type timestamp => Return _ (syntax.Timestamp_constant z)
+          Return (syntax.Mutez_constant (Mk_mutez m))
+        | Comparable_type timestamp => Return (syntax.Timestamp_constant z)
         | _ => Failed _ (Typing _ (d, ty))
         end
     | String_constant s =>
       fun ty =>
         match ty with
-        | Comparable_type string => Return _ (syntax.String_constant s)
-        | signature => Return _ (syntax.Signature_constant s)
-        | key => Return _ (syntax.Key_constant s)
-        | Comparable_type key_hash => Return _ (syntax.Key_hash_constant s)
+        | Comparable_type string => Return (syntax.String_constant s)
+        | signature => Return (syntax.Signature_constant s)
+        | key => Return (syntax.Key_constant s)
+        | Comparable_type key_hash => Return (syntax.Key_hash_constant s)
         | contract a =>
           let c := Mk_contract s in
           type_contract_data c a
-        | Comparable_type address => Return _ (syntax.Address_constant (syntax.Mk_address s))
-        | chain_id => Return _ (syntax.Chain_id_constant (syntax.Mk_chain_id s))
+        | Comparable_type address => Return (syntax.Address_constant (syntax.Mk_address s))
+        | chain_id => Return (syntax.Chain_id_constant (syntax.Mk_chain_id s))
         | _ => Failed _ (Typing _ (d, ty))
         end
     | Bytes_constant s =>
       fun ty =>
         match ty with
-        | Comparable_type bytes => Return _ (syntax.Bytes_constant s)
+        | Comparable_type bytes => Return (syntax.Bytes_constant s)
         | _ => Failed _ (Typing _ (d, ty))
         end
     | Unit =>
       fun ty =>
         match ty with
-        | unit => Return _ syntax.Unit
+        | unit => Return syntax.Unit
         | _ => Failed _ (Typing _ (d, ty))
         end
     | True_ =>
       fun ty =>
         match ty with
-        | Comparable_type bool => Return _ syntax.True_
+        | Comparable_type bool => Return syntax.True_
         | _ => Failed _ (Typing _ (d, ty))
         end
     | False_ =>
       fun ty =>
         match ty with
-        | Comparable_type bool => Return _ syntax.False_
+        | Comparable_type bool => Return syntax.False_
         | _ => Failed _ (Typing _ (d, ty))
         end
     | Pair x y =>
@@ -262,7 +262,7 @@ Module Typer(C:ContractContext).
         | pair a b =>
           let! x := type_data x a in
           let! y := type_data y b in
-          Return _ (syntax.Pair x y)
+          Return (syntax.Pair x y)
         | _ => Failed _ (Typing _ (d, ty))
         end
     | Left x =>
@@ -270,7 +270,7 @@ Module Typer(C:ContractContext).
         match ty with
         | or a b =>
           let! x := type_data x a in
-          Return _ (syntax.Left x)
+          Return (syntax.Left x)
         | _ => Failed _ (Typing _ (d, ty))
         end
     | Right y =>
@@ -278,7 +278,7 @@ Module Typer(C:ContractContext).
         match ty with
         | or a b =>
           let! y := type_data y b in
-          Return _ (syntax.Right y)
+          Return (syntax.Right y)
         | _ => Failed _ (Typing _ (d, ty))
         end
     | Some_ x =>
@@ -286,13 +286,13 @@ Module Typer(C:ContractContext).
         match ty with
         | option a =>
           let! x := type_data x a in
-          Return _ (syntax.Some_ x)
+          Return (syntax.Some_ x)
         | _ => Failed _ (Typing _ (d, ty))
         end
     | None_ =>
       fun ty =>
         match ty with
-        | option a => Return _ syntax.None_
+        | option a => Return syntax.None_
         | _ => Failed _ (Typing _ (d, ty))
         end
     | Concrete_seq l =>
@@ -302,40 +302,40 @@ Module Typer(C:ContractContext).
           let! l :=
             (fix type_data_list l :=
               match l with
-              | nil => Return _ nil
+              | nil => Return nil
               | cons x l =>
                 let! x := type_data x a in
                 let! l := type_data_list l in
-                Return _ (cons x l)
+                Return (cons x l)
               end
             ) l in
-          Return _ (syntax.Concrete_list l)
+          Return (syntax.Concrete_list l)
         | set a =>
           let! l :=
             (fix type_data_list l :=
               match l with
-              | nil => Return _ nil
+              | nil => Return nil
               | cons x l =>
                 let! x := type_data x a in
                 let! l := type_data_list l in
-                Return _ (cons x l)
+                Return (cons x l)
               end
             ) l in
-          Return _ (syntax.Concrete_set l)
+          Return (syntax.Concrete_set l)
         | map a b =>
           let! l :=
             (fix type_data_list l :=
               match l with
-              | nil => Return _ nil
+              | nil => Return nil
               | cons (Elt x y) l =>
                 let! x := type_data x a in
                 let! y := type_data y b in
                 let! l := type_data_list l in
-                Return _ (cons (syntax.Elt _ _ x y) l)
+                Return (cons (syntax.Elt _ _ x y) l)
               | _ => Failed _ (Typing _ (d, ty))
               end
             ) l in
-          Return _ (syntax.Concrete_map l)
+          Return (syntax.Concrete_map l)
         | _ => Failed _ (Typing _ (d, ty))
         end
     | Instruction i =>
@@ -343,7 +343,7 @@ Module Typer(C:ContractContext).
         match ty with
         | lambda a b =>
           let! existT _ tff i := type_check_instruction type_instruction i (cons a nil) (cons b nil) in
-          Return _ (syntax.Instruction _ i)
+          Return (syntax.Instruction _ i)
         | _ => Failed _ (Typing _ (d, ty))
         end
     | d => fun ty => Failed _ (Typing _ (d, ty))
@@ -352,16 +352,16 @@ Module Typer(C:ContractContext).
   with
   type_instruction {self_type} i A {struct i} : M (typer_result (self_type := self_type) A) :=
     match i, A with
-    | NOOP, A => Return _ (Inferred_type _ _ syntax.NOOP)
-    | FAILWITH, a :: A => Return _ (Any_type _ (fun B => syntax.FAILWITH))
+    | NOOP, A => Return (Inferred_type _ _ syntax.NOOP)
+    | FAILWITH, a :: A => Return (Any_type _ (fun B => syntax.FAILWITH))
     | SEQ i1 i2, A =>
       let! existT _ B i1 := type_instruction_no_tail_fail type_instruction i1 A in
       let! r2 := type_instruction i2 B in
       match r2 with
       | Inferred_type _ C i2 =>
-        Return _ (Inferred_type _ _ (syntax.SEQ i1 i2))
+        Return (Inferred_type _ _ (syntax.SEQ i1 i2))
       | Any_type _ i2 =>
-        Return _ (Any_type _ (fun C => syntax.SEQ i1 (i2 C)))
+        Return (Any_type _ (fun C => syntax.SEQ i1 (i2 C)))
       end
     | IF_ i1 i2, Comparable_type bool :: A =>
       type_branches type_instruction i1 i2 _ _ _ (fun B tffa tffb => syntax.IF_)
@@ -376,236 +376,236 @@ Module Typer(C:ContractContext).
     | LOOP i, Comparable_type bool :: A =>
       let! i := type_check_instruction_no_tail_fail
         type_instruction i A (bool ::: A) in
-      Return _ (Inferred_type _ _ (syntax.LOOP i))
+      Return (Inferred_type _ _ (syntax.LOOP i))
     | LOOP_LEFT i, or a b :: A =>
       let! i := type_check_instruction_no_tail_fail
         type_instruction i (a :: A) (or a b :: A) in
-      Return _ (Inferred_type _ _ (syntax.LOOP_LEFT i))
+      Return (Inferred_type _ _ (syntax.LOOP_LEFT i))
     | EXEC, a :: lambda a' b :: B =>
       let A := a :: lambda a' b :: B in
       let A' := a :: lambda a b :: B in
       let! i := instruction_cast_domain A' A _ syntax.EXEC in
-      Return _ (Inferred_type _ _ i)
+      Return (Inferred_type _ _ i)
     | APPLY, a :: lambda (pair a' b) c :: B =>
       let A := a :: lambda (pair a' b) c :: B in
       let A' := a :: lambda (pair a b) c :: B in
       (if is_packable a as b return is_packable a = b -> _
        then fun i =>
         let! i := instruction_cast_domain A' A _ (@syntax.APPLY _ _ _ _ _ (IT_eq_rev _ i)) in
-        Return _ (Inferred_type _ _ i)
+        Return (Inferred_type _ _ i)
        else fun _ => Failed _ (Typing _ "APPLY"%string)) eq_refl
     | DUP, a :: A =>
-      Return _ (Inferred_type _ _ syntax.DUP)
+      Return (Inferred_type _ _ syntax.DUP)
     | SWAP, a :: b :: A =>
-      Return _ (Inferred_type _ _ syntax.SWAP)
+      Return (Inferred_type _ _ syntax.SWAP)
     | PUSH a v, A =>
       let! d := type_data v a in
-      Return _ (Inferred_type _ _ (syntax.PUSH a d))
-    | UNIT, A => Return _ (Inferred_type _ _ syntax.UNIT)
+      Return (Inferred_type _ _ (syntax.PUSH a d))
+    | UNIT, A => Return (Inferred_type _ _ syntax.UNIT)
     | LAMBDA a b i, A =>
       let! existT _ tff i :=
         type_check_instruction type_instruction i (a :: nil) (b :: nil) in
-      Return _ (Inferred_type _ _ (syntax.LAMBDA a b i))
+      Return (Inferred_type _ _ (syntax.LAMBDA a b i))
     | EQ, Comparable_type int :: A =>
-      Return _ (Inferred_type _ _ syntax.EQ)
+      Return (Inferred_type _ _ syntax.EQ)
     | NEQ, Comparable_type int :: A =>
-      Return _ (Inferred_type _ _ syntax.NEQ)
+      Return (Inferred_type _ _ syntax.NEQ)
     | LT, Comparable_type int :: A =>
-      Return _ (Inferred_type _ _ syntax.LT)
+      Return (Inferred_type _ _ syntax.LT)
     | GT, Comparable_type int :: A =>
-      Return _ (Inferred_type _ _ syntax.GT)
+      Return (Inferred_type _ _ syntax.GT)
     | LE, Comparable_type int :: A =>
-      Return _ (Inferred_type _ _ syntax.LE)
+      Return (Inferred_type _ _ syntax.LE)
     | GE, Comparable_type int :: A =>
-      Return _ (Inferred_type _ _ syntax.GE)
+      Return (Inferred_type _ _ syntax.GE)
     | OR, Comparable_type bool :: Comparable_type bool :: A =>
-      Return _ (Inferred_type _ _ (@syntax.OR _ _ syntax.bitwise_bool _))
+      Return (Inferred_type _ _ (@syntax.OR _ _ syntax.bitwise_bool _))
     | OR, Comparable_type nat :: Comparable_type nat :: A =>
-      Return _ (Inferred_type _ _ (@syntax.OR _ _ syntax.bitwise_nat _))
+      Return (Inferred_type _ _ (@syntax.OR _ _ syntax.bitwise_nat _))
     | AND, Comparable_type bool :: Comparable_type bool :: A =>
-      Return _ (Inferred_type _ _ (@syntax.AND _ _ syntax.bitwise_bool _))
+      Return (Inferred_type _ _ (@syntax.AND _ _ syntax.bitwise_bool _))
     | AND, Comparable_type nat :: Comparable_type nat :: A =>
-      Return _ (Inferred_type _ _ (@syntax.AND _ _ syntax.bitwise_nat _))
+      Return (Inferred_type _ _ (@syntax.AND _ _ syntax.bitwise_nat _))
     | XOR, Comparable_type bool :: Comparable_type bool :: A =>
-      Return _ (Inferred_type _ _ (@syntax.XOR _ _ syntax.bitwise_bool _))
+      Return (Inferred_type _ _ (@syntax.XOR _ _ syntax.bitwise_bool _))
     | XOR, Comparable_type nat :: Comparable_type nat :: A =>
-      Return _ (Inferred_type _ _ (@syntax.XOR _ _ syntax.bitwise_nat _))
+      Return (Inferred_type _ _ (@syntax.XOR _ _ syntax.bitwise_nat _))
     | NOT, Comparable_type bool :: A =>
-      Return _ (Inferred_type _ _ (@syntax.NOT _ _ syntax.not_bool _))
+      Return (Inferred_type _ _ (@syntax.NOT _ _ syntax.not_bool _))
     | NOT, Comparable_type nat :: A =>
-      Return _ (Inferred_type _ _ (@syntax.NOT _ _ syntax.not_nat _))
+      Return (Inferred_type _ _ (@syntax.NOT _ _ syntax.not_nat _))
     | NOT, Comparable_type int :: A =>
-      Return _ (Inferred_type _ _ (@syntax.NOT _ _ syntax.not_int _))
+      Return (Inferred_type _ _ (@syntax.NOT _ _ syntax.not_int _))
     | NEG, Comparable_type nat :: A =>
-      Return _ (Inferred_type _ _ (@syntax.NEG _ _ syntax.neg_nat _))
+      Return (Inferred_type _ _ (@syntax.NEG _ _ syntax.neg_nat _))
     | NEG, Comparable_type int :: A =>
-      Return _ (Inferred_type _ _ (@syntax.NEG _ _ syntax.neg_int _))
+      Return (Inferred_type _ _ (@syntax.NEG _ _ syntax.neg_int _))
     | ABS, Comparable_type int :: A =>
-      Return _ (Inferred_type _ _ syntax.ABS)
+      Return (Inferred_type _ _ syntax.ABS)
     | INT, Comparable_type nat :: A =>
-      Return _ (Inferred_type _ _ syntax.INT)
+      Return (Inferred_type _ _ syntax.INT)
     | ISNAT, Comparable_type int :: A =>
-      Return _ (Inferred_type _ _ syntax.ISNAT)
+      Return (Inferred_type _ _ syntax.ISNAT)
     | ADD, Comparable_type nat :: Comparable_type nat :: A =>
-      Return _ (Inferred_type _ _ (@syntax.ADD _ _ _ syntax.add_nat_nat _))
+      Return (Inferred_type _ _ (@syntax.ADD _ _ _ syntax.add_nat_nat _))
     | ADD, Comparable_type nat :: Comparable_type int :: A =>
-      Return _ (Inferred_type _ _ (@syntax.ADD _ _ _ syntax.add_nat_int _))
+      Return (Inferred_type _ _ (@syntax.ADD _ _ _ syntax.add_nat_int _))
     | ADD, Comparable_type int :: Comparable_type nat :: A =>
-      Return _ (Inferred_type _ _ (@syntax.ADD _ _ _ syntax.add_int_nat _))
+      Return (Inferred_type _ _ (@syntax.ADD _ _ _ syntax.add_int_nat _))
     | ADD, Comparable_type int :: Comparable_type int :: A =>
-      Return _ (Inferred_type _ _ (@syntax.ADD _ _ _ syntax.add_int_int _))
+      Return (Inferred_type _ _ (@syntax.ADD _ _ _ syntax.add_int_int _))
     | ADD, Comparable_type timestamp :: Comparable_type int :: A =>
-      Return _ (Inferred_type _ _ (@syntax.ADD _ _ _ syntax.add_timestamp_int _))
+      Return (Inferred_type _ _ (@syntax.ADD _ _ _ syntax.add_timestamp_int _))
     | ADD, Comparable_type int :: Comparable_type timestamp :: A =>
-      Return _ (Inferred_type _ _ (@syntax.ADD _ _ _ syntax.add_int_timestamp _))
+      Return (Inferred_type _ _ (@syntax.ADD _ _ _ syntax.add_int_timestamp _))
     | ADD, Comparable_type mutez :: Comparable_type mutez :: A =>
-      Return _ (Inferred_type _ _ (@syntax.ADD _ _ _ syntax.add_tez_tez _))
+      Return (Inferred_type _ _ (@syntax.ADD _ _ _ syntax.add_tez_tez _))
     | SUB, Comparable_type nat :: Comparable_type nat :: A =>
-      Return _ (Inferred_type _ _ (@syntax.SUB _ _ _ syntax.sub_nat_nat _))
+      Return (Inferred_type _ _ (@syntax.SUB _ _ _ syntax.sub_nat_nat _))
     | SUB, Comparable_type nat :: Comparable_type int :: A =>
-      Return _ (Inferred_type _ _ (@syntax.SUB _ _ _ syntax.sub_nat_int _))
+      Return (Inferred_type _ _ (@syntax.SUB _ _ _ syntax.sub_nat_int _))
     | SUB, Comparable_type int :: Comparable_type nat :: A =>
-      Return _ (Inferred_type _ _ (@syntax.SUB _ _ _ syntax.sub_int_nat _))
+      Return (Inferred_type _ _ (@syntax.SUB _ _ _ syntax.sub_int_nat _))
     | SUB, Comparable_type int :: Comparable_type int :: A =>
-      Return _ (Inferred_type _ _ (@syntax.SUB _ _ _ syntax.sub_int_int _))
+      Return (Inferred_type _ _ (@syntax.SUB _ _ _ syntax.sub_int_int _))
     | SUB, Comparable_type timestamp :: Comparable_type int :: A =>
-      Return _ (Inferred_type _ _ (@syntax.SUB _ _ _ syntax.sub_timestamp_int _))
+      Return (Inferred_type _ _ (@syntax.SUB _ _ _ syntax.sub_timestamp_int _))
     | SUB, Comparable_type timestamp :: Comparable_type timestamp :: A =>
-      Return _ (Inferred_type _ _ (@syntax.SUB _ _ _ syntax.sub_timestamp_timestamp _))
+      Return (Inferred_type _ _ (@syntax.SUB _ _ _ syntax.sub_timestamp_timestamp _))
     | SUB, Comparable_type mutez :: Comparable_type mutez :: A =>
-      Return _ (Inferred_type _ _ (@syntax.SUB _ _ _ syntax.sub_tez_tez _))
+      Return (Inferred_type _ _ (@syntax.SUB _ _ _ syntax.sub_tez_tez _))
     | MUL, Comparable_type nat :: Comparable_type nat :: A =>
-      Return _ (Inferred_type _ _ (@syntax.MUL _ _ _ syntax.mul_nat_nat _))
+      Return (Inferred_type _ _ (@syntax.MUL _ _ _ syntax.mul_nat_nat _))
     | MUL, Comparable_type nat :: Comparable_type int :: A =>
-      Return _ (Inferred_type _ _ (@syntax.MUL _ _ _ syntax.mul_nat_int _))
+      Return (Inferred_type _ _ (@syntax.MUL _ _ _ syntax.mul_nat_int _))
     | MUL, Comparable_type int :: Comparable_type nat :: A =>
-      Return _ (Inferred_type _ _ (@syntax.MUL _ _ _ syntax.mul_int_nat _))
+      Return (Inferred_type _ _ (@syntax.MUL _ _ _ syntax.mul_int_nat _))
     | MUL, Comparable_type int :: Comparable_type int :: A =>
-      Return _ (Inferred_type _ _ (@syntax.MUL _ _ _ syntax.mul_int_int _))
+      Return (Inferred_type _ _ (@syntax.MUL _ _ _ syntax.mul_int_int _))
     | MUL, Comparable_type mutez :: Comparable_type nat :: A =>
-      Return _ (Inferred_type _ _ (@syntax.MUL _ _ _ syntax.mul_tez_nat _))
+      Return (Inferred_type _ _ (@syntax.MUL _ _ _ syntax.mul_tez_nat _))
     | MUL, Comparable_type nat :: Comparable_type mutez :: A =>
-      Return _ (Inferred_type _ _ (@syntax.MUL _ _ _ syntax.mul_nat_tez _))
+      Return (Inferred_type _ _ (@syntax.MUL _ _ _ syntax.mul_nat_tez _))
     | EDIV, Comparable_type nat :: Comparable_type nat :: A =>
-      Return _ (Inferred_type _ _ (@syntax.EDIV _ _ _ syntax.ediv_nat_nat _))
+      Return (Inferred_type _ _ (@syntax.EDIV _ _ _ syntax.ediv_nat_nat _))
     | EDIV, Comparable_type nat :: Comparable_type int :: A =>
-      Return _ (Inferred_type _ _ (@syntax.EDIV _ _ _ syntax.ediv_nat_int _))
+      Return (Inferred_type _ _ (@syntax.EDIV _ _ _ syntax.ediv_nat_int _))
     | EDIV, Comparable_type int :: Comparable_type nat :: A =>
-      Return _ (Inferred_type _ _ (@syntax.EDIV _ _ _ syntax.ediv_int_nat _))
+      Return (Inferred_type _ _ (@syntax.EDIV _ _ _ syntax.ediv_int_nat _))
     | EDIV, Comparable_type int :: Comparable_type int :: A =>
-      Return _ (Inferred_type _ _ (@syntax.EDIV _ _ _ syntax.ediv_int_int _))
+      Return (Inferred_type _ _ (@syntax.EDIV _ _ _ syntax.ediv_int_int _))
     | EDIV, Comparable_type mutez :: Comparable_type nat :: A =>
-      Return _ (Inferred_type _ _ (@syntax.EDIV _ _ _ syntax.ediv_tez_nat _))
+      Return (Inferred_type _ _ (@syntax.EDIV _ _ _ syntax.ediv_tez_nat _))
     | EDIV, Comparable_type mutez :: Comparable_type mutez :: A =>
-      Return _ (Inferred_type _ _ (@syntax.EDIV _ _ _ syntax.ediv_tez_tez _))
+      Return (Inferred_type _ _ (@syntax.EDIV _ _ _ syntax.ediv_tez_tez _))
     | LSL, Comparable_type nat :: Comparable_type nat :: A =>
-      Return _ (Inferred_type _ _ syntax.LSL)
+      Return (Inferred_type _ _ syntax.LSL)
     | LSR, Comparable_type nat :: Comparable_type nat :: A =>
-      Return _ (Inferred_type _ _ syntax.LSR)
+      Return (Inferred_type _ _ syntax.LSR)
     | COMPARE, a :: a' :: B =>
       let A := a ::: a' ::: B in
       let! a : comparable_type := as_comparable a in
       let! a' : comparable_type := as_comparable a' in
       let A' := a ::: a ::: B in
       let! i := instruction_cast_domain A' A (int ::: B) (syntax.COMPARE (a := a)) in
-      Return _ (Inferred_type _ _ i)
+      Return (Inferred_type _ _ i)
     | CONCAT, Comparable_type string :: Comparable_type string :: B =>
-      Return _ (Inferred_type _ _ (@syntax.CONCAT _ _ stringlike_string _))
+      Return (Inferred_type _ _ (@syntax.CONCAT _ _ stringlike_string _))
     | CONCAT, Comparable_type bytes :: Comparable_type bytes :: B =>
-      Return _ (Inferred_type _ _ (@syntax.CONCAT _ _ stringlike_bytes _))
+      Return (Inferred_type _ _ (@syntax.CONCAT _ _ stringlike_bytes _))
     | CONCAT, list (Comparable_type string) :: B =>
-      Return _ (Inferred_type _ _ (@syntax.CONCAT_list _ _ stringlike_string _))
+      Return (Inferred_type _ _ (@syntax.CONCAT_list _ _ stringlike_string _))
     | CONCAT, list (Comparable_type bytes) :: B =>
-      Return _ (Inferred_type _ _ (@syntax.CONCAT_list _ _ stringlike_bytes _))
+      Return (Inferred_type _ _ (@syntax.CONCAT_list _ _ stringlike_bytes _))
     | SIZE, set a :: A =>
-      Return _ (Inferred_type _ _ (@syntax.SIZE _ _ (size_set a) _))
+      Return (Inferred_type _ _ (@syntax.SIZE _ _ (size_set a) _))
     | SIZE, cons (list a) A =>
-      Return _ (Inferred_type _ _ (@syntax.SIZE _ _ (size_list a) _))
+      Return (Inferred_type _ _ (@syntax.SIZE _ _ (size_list a) _))
     | SIZE, cons (map a b) A =>
-      Return _ (Inferred_type _ _ (@syntax.SIZE _ _ (size_map a b) _))
+      Return (Inferred_type _ _ (@syntax.SIZE _ _ (size_map a b) _))
     | SIZE, Comparable_type string :: A =>
-      Return _ (Inferred_type _ _ (@syntax.SIZE _ _ size_string _))
+      Return (Inferred_type _ _ (@syntax.SIZE _ _ size_string _))
     | SIZE, Comparable_type bytes :: A =>
-      Return _ (Inferred_type _ _ (@syntax.SIZE _ _ size_bytes _))
+      Return (Inferred_type _ _ (@syntax.SIZE _ _ size_bytes _))
     | SLICE, Comparable_type nat :: Comparable_type nat :: Comparable_type string :: A =>
-      Return _ (Inferred_type _ _ (@syntax.SLICE _ _ stringlike_string _))
+      Return (Inferred_type _ _ (@syntax.SLICE _ _ stringlike_string _))
     | SLICE, Comparable_type nat :: Comparable_type nat :: Comparable_type bytes :: A =>
-      Return _ (Inferred_type _ _ (@syntax.SLICE _ _ stringlike_bytes _))
+      Return (Inferred_type _ _ (@syntax.SLICE _ _ stringlike_bytes _))
     | PAIR, a :: b :: A =>
-      Return _ (Inferred_type _ _ syntax.PAIR)
+      Return (Inferred_type _ _ syntax.PAIR)
     | CAR, pair a b :: A =>
-      Return _ (Inferred_type _ _ syntax.CAR)
+      Return (Inferred_type _ _ syntax.CAR)
     | CDR, pair a b :: A =>
-      Return _ (Inferred_type _ _ syntax.CDR)
+      Return (Inferred_type _ _ syntax.CDR)
     | EMPTY_SET c, A =>
-      Return _ (Inferred_type _ _ (syntax.EMPTY_SET c))
+      Return (Inferred_type _ _ (syntax.EMPTY_SET c))
     | MEM, elt' :: set elt :: B =>
       let A := elt' :: set elt :: B in
       let A' := elt ::: set elt :: B in
       let! i := instruction_cast_domain
         A' A _ (@syntax.MEM _ _ _ (mem_set elt) _) in
-      Return _ (Inferred_type _ _ i)
+      Return (Inferred_type _ _ i)
     | MEM, kty' :: map kty vty :: B =>
       let A := kty' :: map kty vty :: B in
       let A' := kty ::: map kty vty :: B in
       let! i := instruction_cast_domain
         A' A _ (@syntax.MEM _ _ _ (mem_map kty vty) _) in
-      Return _ (Inferred_type _ _ i)
+      Return (Inferred_type _ _ i)
     | MEM, kty' :: big_map kty vty :: B =>
       let A := kty' :: big_map kty vty :: B in
       let A' := kty ::: big_map kty vty :: B in
       let! i := instruction_cast_domain
         A' A _ (@syntax.MEM _ _ _ (mem_bigmap kty vty) _) in
-      Return _ (Inferred_type _ _ i)
+      Return (Inferred_type _ _ i)
     | UPDATE, elt' :: Comparable_type bool :: set elt :: B =>
       let A := elt' ::: bool ::: set elt :: B in
       let A' := elt ::: bool ::: set elt :: B in
       let! i := instruction_cast_domain
         A' A _ (@syntax.UPDATE _ _ _ _ (update_set elt) _) in
-      Return _ (Inferred_type _ _ i)
+      Return (Inferred_type _ _ i)
     | UPDATE, kty' :: option vty' :: map kty vty :: B =>
       let A := kty' ::: option vty' ::: map kty vty :: B in
       let A' := kty ::: option vty ::: map kty vty :: B in
       let! i := instruction_cast_domain
         A' A _ (@syntax.UPDATE _ _ _ _ (update_map kty vty) _) in
-      Return _ (Inferred_type _ _ i)
+      Return (Inferred_type _ _ i)
     | UPDATE, kty' :: option vty' :: big_map kty vty :: B =>
       let A := kty' ::: option vty' ::: big_map kty vty :: B in
       let A' := kty ::: option vty ::: big_map kty vty :: B in
       let! i := instruction_cast_domain
         A' A _ (@syntax.UPDATE _ _ _ _ (update_bigmap kty vty) _) in
-      Return _ (Inferred_type _ _ i)
+      Return (Inferred_type _ _ i)
     | ITER i, list a :: A =>
       let! i := type_check_instruction_no_tail_fail type_instruction i (a :: A) A in
-      Return _ (Inferred_type _ _ (syntax.ITER i))
+      Return (Inferred_type _ _ (syntax.ITER i))
     | ITER i, set a :: A =>
       let! i := type_check_instruction_no_tail_fail type_instruction i (a ::: A) A in
-      Return _ (Inferred_type _ _ (syntax.ITER i))
+      Return (Inferred_type _ _ (syntax.ITER i))
     | ITER i, map kty vty :: A =>
       let! i := type_check_instruction_no_tail_fail type_instruction i (pair kty vty :: A) A in
-      Return _ (Inferred_type _ _ (syntax.ITER i))
+      Return (Inferred_type _ _ (syntax.ITER i))
     | EMPTY_MAP kty vty, A =>
-      Return _ (Inferred_type _ _ (syntax.EMPTY_MAP kty vty))
+      Return (Inferred_type _ _ (syntax.EMPTY_MAP kty vty))
     | EMPTY_BIG_MAP kty vty, A =>
-      Return _ (Inferred_type _ _ (syntax.EMPTY_BIG_MAP kty vty))
+      Return (Inferred_type _ _ (syntax.EMPTY_BIG_MAP kty vty))
     | GET, kty' :: map kty vty :: B =>
       let A := kty' :: map kty vty :: B in
       let A' := kty ::: map kty vty :: B in
       let! i := instruction_cast_domain
         A' A _ (@syntax.GET _ _ _ (get_map kty vty) _) in
-      Return _ (Inferred_type _ _ i)
+      Return (Inferred_type _ _ i)
     | GET, kty' :: big_map kty vty :: B =>
       let A := kty' :: big_map kty vty :: B in
       let A' := kty ::: big_map kty vty :: B in
       let! i := instruction_cast_domain
         A' A _ (@syntax.GET _ _ _ (get_bigmap kty vty) _) in
-      Return _ (Inferred_type _ _ i)
+      Return (Inferred_type _ _ i)
     | MAP i, list a :: A =>
       let! r := type_instruction_no_tail_fail type_instruction i (a :: A) in
       match r with
       | existT _ (b :: A') i =>
         let! i := instruction_cast_range (a :: A) (b :: A') (b :: A) i in
-        Return _ (Inferred_type _ _ (syntax.MAP i))
+        Return (Inferred_type _ _ (syntax.MAP i))
       | _ => Failed _ (Typing _ tt)
       end
     | MAP i, map kty vty :: A =>
@@ -613,19 +613,19 @@ Module Typer(C:ContractContext).
       match r with
       | existT _ (b :: A') i =>
         let! i := instruction_cast_range (pair kty vty :: A) (b :: A') (b :: A) i in
-        Return _ (Inferred_type _ _ (syntax.MAP i))
+        Return (Inferred_type _ _ (syntax.MAP i))
       | _ => Failed _ (Typing _ tt)
       end
-    | SOME, a :: A => Return _ (Inferred_type _ _ syntax.SOME)
-    | NONE a, A => Return _ (Inferred_type _ _ (syntax.NONE a))
-    | LEFT b, a :: A => Return _ (Inferred_type _ _ (syntax.LEFT b))
-    | RIGHT a, b :: A => Return _ (Inferred_type _ _ (syntax.RIGHT a))
+    | SOME, a :: A => Return (Inferred_type _ _ syntax.SOME)
+    | NONE a, A => Return (Inferred_type _ _ (syntax.NONE a))
+    | LEFT b, a :: A => Return (Inferred_type _ _ (syntax.LEFT b))
+    | RIGHT a, b :: A => Return (Inferred_type _ _ (syntax.RIGHT a))
     | CONS, a' :: list a :: B =>
       let A := a' :: list a :: B in
       let A' := a :: list a :: B in
       let! i := instruction_cast_domain A' A _ (syntax.CONS) in
-      Return _ (Inferred_type _ _ i)
-    | NIL a, A => Return _ (Inferred_type _ _ (syntax.NIL a))
+      Return (Inferred_type _ _ i)
+    | NIL a, A => Return (Inferred_type _ _ (syntax.NIL a))
     | CREATE_CONTRACT g p i,
       option (Comparable_type key_hash) :: Comparable_type mutez :: g2 :: B =>
       let A :=
@@ -635,62 +635,62 @@ Module Typer(C:ContractContext).
       let! existT _ tff i :=
         type_check_instruction (self_type := Some p) type_instruction i (pair p g :: nil) (pair (list operation) g :: nil) in
       let! i := instruction_cast_domain A' A _ (syntax.CREATE_CONTRACT g p i) in
-      Return _ (Inferred_type _ _ i)
+      Return (Inferred_type _ _ i)
     | TRANSFER_TOKENS, p1 :: Comparable_type mutez :: contract p2 :: B =>
       let A := p1 ::: mutez ::: contract p2 ::: B in
       let A' := p1 ::: mutez ::: contract p1 ::: B in
       let! i := instruction_cast_domain A' A _ syntax.TRANSFER_TOKENS in
-      Return _ (Inferred_type _ _ i)
+      Return (Inferred_type _ _ i)
     | SET_DELEGATE, option (Comparable_type key_hash) :: A =>
-      Return _ (Inferred_type _ _ syntax.SET_DELEGATE)
+      Return (Inferred_type _ _ syntax.SET_DELEGATE)
     | BALANCE, A =>
-      Return _ (Inferred_type _ _ syntax.BALANCE)
+      Return (Inferred_type _ _ syntax.BALANCE)
     | ADDRESS, contract _ :: A =>
-      Return _ (Inferred_type _ _ syntax.ADDRESS)
+      Return (Inferred_type _ _ syntax.ADDRESS)
     | CONTRACT ty, Comparable_type address :: A =>
-      Return _ (Inferred_type _ _ (syntax.CONTRACT ty))
+      Return (Inferred_type _ _ (syntax.CONTRACT ty))
     | SOURCE, A =>
-      Return _ (Inferred_type _ _ syntax.SOURCE)
+      Return (Inferred_type _ _ syntax.SOURCE)
     | SENDER, A =>
-      Return _ (Inferred_type _ _ syntax.SENDER)
+      Return (Inferred_type _ _ syntax.SENDER)
     | SELF, A =>
       match self_type with
-      | Some sty => Return _ (Inferred_type _ _ syntax.SELF)
+      | Some sty => Return (Inferred_type _ _ syntax.SELF)
       | None => Failed _ (Typing _ "SELF is not allowed inside lambdas"%string)
       end
     | AMOUNT, A =>
-      Return _ (Inferred_type _ _ syntax.AMOUNT)
+      Return (Inferred_type _ _ syntax.AMOUNT)
     | IMPLICIT_ACCOUNT, Comparable_type key_hash :: A =>
-      Return _ (Inferred_type _ _ syntax.IMPLICIT_ACCOUNT)
+      Return (Inferred_type _ _ syntax.IMPLICIT_ACCOUNT)
     | NOW, A =>
-      Return _ (Inferred_type _ _ syntax.NOW)
+      Return (Inferred_type _ _ syntax.NOW)
     | PACK, a :: A =>
-      Return _ (Inferred_type _ _ syntax.PACK)
+      Return (Inferred_type _ _ syntax.PACK)
     | UNPACK ty, Comparable_type bytes :: A =>
-      Return _ (Inferred_type _ _ (syntax.UNPACK ty))
+      Return (Inferred_type _ _ (syntax.UNPACK ty))
     | HASH_KEY, key :: A =>
-      Return _ (Inferred_type _ _ syntax.HASH_KEY)
+      Return (Inferred_type _ _ syntax.HASH_KEY)
     | BLAKE2B, Comparable_type bytes :: A =>
-      Return _ (Inferred_type _ _ syntax.BLAKE2B)
+      Return (Inferred_type _ _ syntax.BLAKE2B)
     | SHA256, Comparable_type bytes :: A =>
-      Return _ (Inferred_type _ _ syntax.SHA256)
+      Return (Inferred_type _ _ syntax.SHA256)
     | SHA512, Comparable_type bytes :: A =>
-      Return _ (Inferred_type _ _ syntax.SHA512)
+      Return (Inferred_type _ _ syntax.SHA512)
     | CHECK_SIGNATURE, key :: signature :: Comparable_type bytes :: A =>
-      Return _ (Inferred_type _ _ syntax.CHECK_SIGNATURE)
+      Return (Inferred_type _ _ syntax.CHECK_SIGNATURE)
     | DIG n, A => type_check_dig n _
     | DUG n, A => type_check_dug n _
     | DIP n i, S12 =>
       let! (exist _ S1 H1, S2) := take_n S12 n in
       let! existT _ B i := type_instruction_no_tail_fail type_instruction i S2 in
       let! i := instruction_cast_domain (S1 +++ S2) S12 _ (syntax.DIP n H1 i) in
-      Return _ (Inferred_type S12 (S1 +++ B) i)
+      Return (Inferred_type S12 (S1 +++ B) i)
     | DROP n, S12 =>
       let! (exist _ S1 H1, S2) := take_n S12 n in
       let! i := instruction_cast_domain (S1 +++ S2) S12 _ (syntax.DROP n H1) in
-      Return _ (Inferred_type S12 S2 i)
+      Return (Inferred_type S12 S2 i)
     | CHAIN_ID, _ =>
-      Return _ (Inferred_type _ _ syntax.CHAIN_ID)
+      Return (Inferred_type _ _ syntax.CHAIN_ID)
     | _, _ => Failed _ (Typing _ (i, A))
     end.
 End Typer.
