src/contracts_coq/return_to_sender.v
@@ -83,7 +83,7 @@ Qed.
 Lemma return_to_sender_correct :
   forall (ops : data (list operation)) (fuel : Datatypes.nat),
   fuel >= 42 ->
-  eval env return_to_sender fuel ((tt, tt), tt) = Return _ ((ops, tt), tt)
+  eval env return_to_sender fuel ((tt, tt), tt) = Return ((ops, tt), tt)
   <->
   (amount env = (0 ~Mutez) /\ ops = nil) \/
   (amount env <> (0 ~Mutez) /\
